Distinguish between pure and impure reactions (Part 1)

Runtime/Reaction.lean
@@ -31,8 +31,8 @@ structure Output (σPortEffect σActionEffect σState : Interface.Scheme) (min :
   state  : Interface σState
   events : SortedArray (Event σActionEffect min) := #[]#
 
-def _root_.ReactionM (σPortSource σPortEffect σActionSource σActionEffect σState σParam : Interface.Scheme) (α : Type) := 
-  (input : Input σPortSource σActionSource σState σParam) → IO (Output σPortEffect σActionEffect σState input.time × α)
+abbrev _root_.ReactionT (σPortSource σPortEffect σActionSource σActionEffect σState σParam : Interface.Scheme) (m : Type → Type) (α : Type) := 
+  (input : Input σPortSource σActionSource σState σParam) → m (Output σPortEffect σActionEffect σState input.time × α)
 
 def Output.merge (o₁ o₂ : ReactionM.Output σPortEffect σActionEffect σState time) : Output σPortEffect σActionEffect σState time where
   ports  := o₁.ports.merge o₂.ports
@@ -60,7 +60,9 @@ def Input.noop (input : Input σPortSource σActionSource σState σParam) : Out
 theorem Input.noop_ports_isEmpty (input : Input σPortSource σActionSource σState σParam) {σPortEffect σActionEffect} : 
   input.noop (σPortEffect := σPortEffect) (σActionEffect := σActionEffect) |>.ports.isEmpty := rfl
 
-instance : Monad (ReactionM σPortSource σPortEffect σActionSource σActionEffect σState σParam) where
+variable [Monad m]
+
+instance : Monad (ReactionT σPortSource σPortEffect σActionSource σActionEffect σState σParam m) where
   pure a input := do
     let output := input.noop
     return (output, a)
@@ -79,46 +81,46 @@ instance : Monad (ReactionM σPortSource σPortEffect σActionSource σActionEff
     let output := output₁.merge output₂
     return (output, b)
 
-instance : MonadLift IO (ReactionM σPortSource σPortEffect σActionSource σActionEffect σState σParam) where
+instance : MonadLift IO (ReactionT σPortSource σPortEffect σActionSource σActionEffect σState σParam IO) where
   monadLift io input world := 
     match io world with 
     | .error e world' => .error e world'
     | .ok    a world' => .ok (input.noop, a) world'
 
-def getInput (port : σPortSource.vars) : ReactionM σPortSource σPortEffect σActionSource σActionEffect σState σParam (Option $ σPortSource.type port) :=
+def getInput (port : σPortSource.vars) : ReactionT σPortSource σPortEffect σActionSource σActionEffect σState σParam m (Option $ σPortSource.type port) :=
   fun input => return (input.noop, input.ports port)
   
-def getState (stv : σState.vars) : ReactionM σPortSource σPortEffect σActionSource σActionEffect σState σParam (σState.type stv) :=
+def getState (stv : σState.vars) : ReactionT σPortSource σPortEffect σActionSource σActionEffect σState σParam m (σState.type stv) :=
   fun input => return (input.noop, input.state stv)
 
-def getAction (action : σActionSource.vars) : ReactionM σPortSource σPortEffect σActionSource σActionEffect σState σParam (Option $ σActionSource.type action) :=
+def getAction (action : σActionSource.vars) : ReactionT σPortSource σPortEffect σActionSource σActionEffect σState σParam m (Option $ σActionSource.type action) :=
   fun input => return (input.noop, input.actions action)
 
-def getParam (param : σParam.vars) : ReactionM σPortSource σPortEffect σActionSource σActionEffect σState σParam (σParam.type param) :=
+def getParam (param : σParam.vars) : ReactionT σPortSource σPortEffect σActionSource σActionEffect σState σParam m (σParam.type param) :=
   fun input => return (input.noop, input.params param)
 
-def getTag : ReactionM σPortSource σPortEffect σActionSource σActionEffect σState σParam Tag := 
+def getTag : ReactionT σPortSource σPortEffect σActionSource σActionEffect σState σParam m Tag := 
   fun input => return (input.noop, input.tag)
 
-def getLogicalTime : ReactionM σPortSource σPortEffect σActionSource σActionEffect σState σParam Time := do
+def getLogicalTime : ReactionT σPortSource σPortEffect σActionSource σActionEffect σState σParam m Time := do
   return (← getTag).time
 
-def getPhysicalTime : ReactionM σPortSource σPortEffect σActionSource σActionEffect σState σParam Time :=
+def getPhysicalTime : ReactionT σPortSource σPortEffect σActionSource σActionEffect σState σParam IO Time :=
   fun input => return (input.noop, (← Time.now) - input.physicalOffset)
 
-def setOutput (port : σPortEffect.vars) (v : σPortEffect.type port) : ReactionM σPortSource σPortEffect σActionSource σActionEffect σState σParam Unit :=
+def setOutput (port : σPortEffect.vars) (v : σPortEffect.type port) : ReactionT σPortSource σPortEffect σActionSource σActionEffect σState σParam m Unit :=
   fun input => 
     let ports := fun p => if h : p = port then some (h ▸ v) else none
     let output := { ports := ports, state := input.state }
     return (output, ())
 
-def setState (stv : σState.vars) (v : σState.type stv) : ReactionM σPortSource σPortEffect σActionSource σActionEffect σState σParam Unit :=
+def setState (stv : σState.vars) (v : σState.type stv) : ReactionT σPortSource σPortEffect σActionSource σActionEffect σState σParam m Unit :=
   fun input =>
     let state := fun s => if h : s = stv then h ▸ v else input.state s
     let output := { state := state }
     return (output, ())
 
-def schedule (action : σActionEffect.vars) (delay : Duration) (v : σActionEffect.type action) : ReactionM σPortSource σPortEffect σActionSource σActionEffect σState σParam Unit := 
+def schedule (action : σActionEffect.vars) (delay : Duration) (v : σActionEffect.type action) : ReactionT σPortSource σPortEffect σActionSource σActionEffect σState σParam m Unit := 
   fun input => 
     let time := input.time.advance delay
     let event := { action, time, value := v }
@@ -134,7 +136,7 @@ inductive Reaction.Trigger (Port Action Timer : Type)
   | action (a : Action)
   | timer (t : Timer)
 
-structure _root_.Reaction where
+structure _root_.Reaction (m : Type → Type) where
   portSources   : Interface.Scheme
   portEffects   : Interface.Scheme
   actionSources : Interface.Scheme
@@ -143,20 +145,20 @@ structure _root_.Reaction where
   params        : Interface.Scheme
   timers        : Type
   triggers      : Array (Reaction.Trigger portSources.vars actionSources.vars timers)
-  body          : ReactionM portSources portEffects actionSources actionEffects state params Unit
+  body          : ReactionT portSources portEffects actionSources actionEffects state params m Unit
 
 namespace Reaction
 
-abbrev inputType (rcn : Reaction) :=
+abbrev inputType (rcn : Reaction m) :=
   ReactionM.Input rcn.portSources rcn.actionSources rcn.state rcn.params
 
-abbrev outputType (rcn : Reaction) :=
+abbrev outputType (rcn : Reaction m) :=
   ReactionM.Output rcn.portEffects rcn.actionEffects rcn.state 
 
-abbrev bodyType (rcn : Reaction) :=
-  ReactionM rcn.portSources rcn.portEffects rcn.actionSources rcn.actionEffects rcn.state rcn.params Unit
+abbrev bodyType (rcn : Reaction m) :=
+  ReactionT rcn.portSources rcn.portEffects rcn.actionSources rcn.actionEffects rcn.state rcn.params m Unit
 
-def run (rcn : Reaction) (input : rcn.inputType) : IO (rcn.outputType input.time) := 
+def run [Functor m] (rcn : Reaction m) (input : rcn.inputType) : m (rcn.outputType input.time) := 
   Prod.fst <$> rcn.body input
 
 end Reaction
