Runtime/Verification/ReactionMSat.lean
@@ -1,13 +1,7 @@
 import Runtime.Reaction
 
-instance : LawfulMonad IO := sorry
-
+/-
 namespace ReactionM
-
--- https://leanprover.zulipchat.com/#narrow/stream/270676-lean4/topic/SatisfiesM.2Eand
-theorem SatisfiesM.and [Functor m] [LawfulFunctor m] {x : m α} :
-  (SatisfiesM p x) → (SatisfiesM q x) → SatisfiesM (fun a => p a ∧ q a) x := by
-  sorry
 
 protected def Sat
   (input : Input σPortSource σActionSource σState σParam)
@@ -47,3 +41,4 @@ theorem Sat.and :
   SatisfiesM.and
 
 end ReactionM
+-/
